Replace elab_typ with a syntactic relation between source and target types

rupicola/stlc_v2/Compiler.fst
@@ -7,53 +7,22 @@ open FStar.List.Tot
 
 open STLC
 open SyntacticTypes
-open SemanticTyping
 open EquivRel
 
 class compile_typ (s:Type) = {
   [@@@no_method] t : typ;
-  [@@@no_method] eq : squash (elab_typ t == s);
-  (** CA: can this equality become problematic when
-          `typ` will encode types that elaborate to
-          refined types, arrows with pre-post conditions, and monadic arrows? **)
+  [@@@no_method] r : rtyp t s;
   (** CA: To get rid of the equality, one would have to find different
-          definitions for `get_v'` and redefine the `equiv` relation. **)
+          definitions for `get_v'`. **)
 }
 
-instance compile_typ_unit : compile_typ unit = { t = TUnit; eq = () }
-instance compile_typ_bool : compile_typ bool = { t = TBool; eq = () }
+instance compile_typ_unit : compile_typ unit = { t = TUnit; r = RUnit }
+instance compile_typ_bool : compile_typ bool = { t = TBool; r = RBool }
 instance compile_typ_arrow (s1:Type) (s2:Type) {| c1:compile_typ s1 |} {| c2:compile_typ s2 |} : compile_typ (s1 -> s2) = {
   t = TArr c1.t c2.t;
-  eq = begin
-    let t = TArr c1.t c2.t in
-    assert (elab_typ t == (elab_typ c1.t -> elab_typ c2.t))
-      by (norm [delta_only [`%elab_typ];zeta;iota]);
-    assert (s1 == elab_typ c1.t);
-    assert (s2 == elab_typ c2.t);
-    assert ((s1 -> s2) == elab_typ t) by (
-      rewrite (nth_binder (-1));
-      rewrite (nth_binder (-3))
-    )
-  end }
+  r = RArr c1.r c2.r }
 
-let rec elab_typ_is_compile_typ (t:typ) : compile_typ (elab_typ t) =
-  match t with
-  | TUnit -> compile_typ_unit
-  | TBool -> compile_typ_bool
-  | TArr t1 t2 ->
-    assume (elab_typ t == (elab_typ t1 -> elab_typ t2)); (** I just proved this a few lines above **)
-    compile_typ_arrow (elab_typ t1) (elab_typ t2) #(elab_typ_is_compile_typ t1) #(elab_typ_is_compile_typ t2)
-
-instance elab_typ_is_compile_typ' (t:typ) : compile_typ (elab_typ t) = elab_typ_is_compile_typ t
-
-let rec inverse_elab_typ_compile_typ (t:typ) : Lemma ((elab_typ_is_compile_typ t).t == t) [SMTPat (elab_typ_is_compile_typ t).t] =
-  match t with
-  | TUnit -> ()
-  | TBool -> ()
-  | TArr t1 t2 ->
-    inverse_elab_typ_compile_typ t1;
-    inverse_elab_typ_compile_typ t2;
-    ()
+let pack #s (c:compile_typ s) : typsr = (| c.t, s, c.r |)
 
 // Some tests
 let test0 : compile_typ (unit) = solve
@@ -69,8 +38,8 @@ class compile_exp (#a:Type0) {| ca: compile_typ a |} (g:env) (fs_e:fs_env g -> a
   [@@@no_method] e : (e:exp{fv_in_env g e}); (** expression is closed by g *)
 
   (** The following two lemmas are indepenent one of the other (we don't use one to prove the other). **)
-  [@@@no_method] typing_proof : unit -> Lemma (sem_typing g e ca.t);
-  [@@@no_method] equiv_proof : unit -> Lemma (fs_e `equiv ca.t` e);
+ // [@@@no_method] typing_proof : unit -> Lemma (sem_typing g e ca.t);
+  [@@@no_method] equiv_proof : unit -> Lemma (fs_e `equiv (pack ca)` e);
 }
 
 (** Just a helper typeclass **)
@@ -78,30 +47,25 @@ unfold let compile_closed (#a:Type0) {| ca: compile_typ a |} (s:a) =
   compile_exp #a empty (fun _ -> s)
 
 let lemma_compile_closed_in_equiv_rel (#a:Type0) {| ca:compile_typ a |} (fs_e:a) {| cs:compile_closed #a #ca fs_e |}
-  : Lemma (ca.t ⦂ (fs_e, cs.e) /\ cs.e ⋮ ca.t) =
+  : Lemma (pack ca ⦂ (fs_e, cs.e)) =
   cs.equiv_proof ();
-  equiv_closed_terms #ca.t fs_e cs.e;
-  cs.typing_proof ();
-  lem_sem_typing_closed cs.e ca.t
+  equiv_closed_terms #(pack ca) fs_e cs.e
 
 let lemma_compile_closed_arrow_is_elam #a #b {| ca:compile_typ a |} {| cb:compile_typ b |} (fs_e:a -> b) {| cs:compile_closed #(a -> b) fs_e |}
   : Lemma (ELam? cs.e) = admit ()
 
 instance compile_exp_unit g : compile_exp #unit #solve g (fun _ -> ()) = {
   e = EUnit;
-  typing_proof = (fun () -> typing_rule_unit g);
   equiv_proof = (fun () -> equiv_unit g);
 }
 
 instance compile_exp_true g : compile_exp #bool #solve g (fun _ -> true) = {
   e = ETrue;
-  typing_proof = (fun () -> typing_rule_true g);
   equiv_proof = (fun () -> equiv_true g);
 }
 
 instance compile_exp_false g : compile_exp #bool #solve g (fun _ -> false) = {
   e = EFalse;
-  typing_proof = (fun () -> typing_rule_false g);
   equiv_proof = (fun () -> equiv_false g);
 }
 
@@ -111,34 +75,29 @@ let test_false : compile_closed false = solve
 
 (** get_v' works better with typeclass resolution than get_v **)
 [@"opaque_to_smt"] (** not sure if the right pragma to prevent F* unfolding it during type class resolution **)
-val get_v' : #g:env -> fs_env g -> x:var{Some? (g x)} -> a:Type{a == elab_typ (Some?.v (g x))} -> a
+val get_v' : #g:env -> fs_env g -> x:var{Some? (g x)} -> a:Type{a == get_Type (Some?.v (g x))} -> a
 let get_v' #g fs_s i a =
   get_v #g fs_s i
 
-instance compile_exp_var (a:Type) {| ca:compile_typ a |} (g:env) (x:var{Some? (g x) /\ ca.t == Some?.v (g x)})
+instance compile_exp_var (a:Type) {| ca:compile_typ a |} (g:env) (x:var{Some? (g x) /\ pack ca == Some?.v (g x)})
   : compile_exp #a #ca g (fun fs_s -> get_v' fs_s x a) = {
     e = EVar x;
-    typing_proof = (fun () ->
-      inverse_elab_typ_compile_typ (Some?.v (g x));
-      typing_rule_var g x
-    );
     equiv_proof = (fun () ->
       reveal_opaque (`%get_v') (get_v' #g);
       equiv_var g x);
 }
 
-let test1_var : compile_exp (extend TUnit empty) (fun fs_s -> get_v' fs_s 0 unit) = solve
+let test1_var : compile_exp (extend tunit empty) (fun fs_s -> get_v' fs_s 0 unit) = solve
 
 instance compile_exp_var_shrink1 (** CA: how to make this general? **)
   (a:Type) {| ca:compile_typ a |}
   (g':env)
-  (t:typ)
+  (t:typsr)
   (g:env{g' == extend t g})
-  (x:var{Some? (g x) /\ ca.t == Some?.v (g x)})
+  (x:var{Some? (g x) /\ pack ca == Some?.v (g x)})
   {| ce:compile_exp g' (fun fs_s -> get_v' #g' fs_s (x+1) a) |} (** this is not necessary. I am hoping that it can be modified to be recursive **)
   : compile_exp g' (fun (fs_s:fs_env g') -> get_v' #g (fs_shrink #t #g fs_s) x a) = {
     e = ce.e;
-    typing_proof = ce.typing_proof;
     equiv_proof = (fun () ->
       reveal_opaque (`%get_v') (get_v' #g');
       reveal_opaque (`%get_v') (get_v' #g);
@@ -148,23 +107,22 @@ instance compile_exp_var_shrink1 (** CA: how to make this general? **)
 instance compile_exp_var_shrink2 (** CA: how to make this general? **)
   (a:Type) {| ca:compile_typ a |}
   (g':env)
-  (t1 t2:typ)
+  (t1 t2:typsr)
   (g:env{g' == extend t1 (extend t2 g)})
-  (x:var{Some? (g x) /\ ca.t == Some?.v (g x)})
+  (x:var{Some? (g x) /\ pack ca == Some?.v (g x)})
   {| ce:compile_exp g' (fun fs_s -> get_v' #g' fs_s (x+2) a) |} (** this is not necessary. I am hoping that it can be modified to be recursive **)
   : compile_exp g' (fun (fs_s:fs_env g') -> get_v' #g (fs_shrink #t2 (fs_shrink #t1 fs_s)) x a) = {
     e = ce.e;
-    typing_proof = ce.typing_proof;
     equiv_proof = (fun () ->
       reveal_opaque (`%get_v') (get_v' #g');
       reveal_opaque (`%get_v') (get_v' #g);
       ce.equiv_proof ());
   }
 
-let test2_var : compile_exp (extend TUnit (extend TUnit empty)) (fun fs_s -> get_v' (fs_shrink fs_s) 0 unit) =
+let test2_var : compile_exp (extend tunit (extend tunit empty)) (fun fs_s -> get_v' (fs_shrink fs_s) 0 unit) =
   solve
 
-let test3_var : compile_exp (extend TUnit (extend TUnit (extend TUnit empty))) (fun fs_s -> get_v' (fs_shrink (fs_shrink fs_s)) 0 unit) =
+let test3_var : compile_exp (extend tunit (extend tunit (extend tunit empty))) (fun fs_s -> get_v' (fs_shrink (fs_shrink fs_s)) 0 unit) =
   solve
 
 instance compile_exp_lambda
@@ -172,20 +130,16 @@ instance compile_exp_lambda
   (#a:Type) {| ca: compile_typ a |}
   (#b:Type) {| cb: compile_typ b |}
   (f:fs_env g -> a -> b)
-  {| cf: compile_exp #b #cb (extend ca.t g) (fun fs_s -> f (fs_shrink #ca.t fs_s) (get_v' fs_s 0 a)) |}
+  {| cf: compile_exp #b #cb (extend (pack ca) g) (fun fs_s -> f (fs_shrink #(pack ca) fs_s) (get_v' fs_s 0 a)) |}
   : compile_exp g f = {
   e = begin
-    lem_fv_in_env_lam g ca.t cf.e;
+    lem_fv_in_env_lam g (pack ca) cf.e;
     ELam cf.e
   end;
-  typing_proof = (fun () ->
-    cf.typing_proof ();
-    typing_rule_lam g ca.t cf.e cb.t
-  );
   equiv_proof = (fun () ->
     cf.equiv_proof ();
-    reveal_opaque (`%get_v') (get_v' #(extend ca.t g));
-    equiv_lam g ca.t cf.e cb.t f
+    reveal_opaque (`%get_v') (get_v' #(extend (pack ca) g));
+    equiv_lam g (pack ca) cf.e (pack cb) f
   )
 }
 
@@ -224,15 +178,10 @@ instance compile_exp_app
     lem_fv_in_env_app g cf.e cx.e;
     EApp cf.e cx.e
   end;
-  typing_proof = (fun () ->
-    cf.typing_proof ();
-    cx.typing_proof ();
-    typing_rule_app g cf.e cx.e ca.t cb.t
-  );
   equiv_proof = (fun () ->
     cf.equiv_proof ();
     cx.equiv_proof ();
-    equiv_app g ca.t cb.t cf.e cx.e f x
+    equiv_app g (pack ca) (pack cb) cf.e cx.e f x
   );
 }
 
@@ -268,17 +217,11 @@ instance compile_exp_if
     lem_fv_in_env_if g cco.e cth.e cel.e;
     EIf cco.e cth.e cel.e
   end;
-  typing_proof = (fun () ->
-    cco.typing_proof ();
-    cth.typing_proof ();
-    cel.typing_proof ();
-    typing_rule_if g cco.e cth.e cel.e ca.t
-  );
   equiv_proof = (fun () ->
     cco.equiv_proof ();
     cth.equiv_proof ();
     cel.equiv_proof ();
-    equiv_if g ca.t cco.e cth.e cel.e co th el
+    equiv_if g (pack ca) cco.e cth.e cel.e co th el
   );
 }
 
@@ -294,6 +237,4 @@ let test1_hoc : compile_closed
   #((bool -> bool) -> bool)
   #(compile_typ_arrow _ _ #(compile_typ_arrow _ _ #compile_typ_bool #compile_typ_bool))
   (fun f -> f false) =
- // assume (elab_typ (compile_typ_arrow _ _ #compile_typ_bool #compile_typ_bool).t == (bool -> bool));
-  assume (elab_typ (TArr TBool TBool) == (bool -> bool));
   compile_exp_lambda _ _ #(compile_exp_app _ (fun fs_s -> get_v' fs_s 0 (bool -> bool)) _)
