rupicola/stlc_v2/EquivRel.fst
@@ -3,12 +3,12 @@ module EquivRel
 open FStar.FunctionalExtensionality
 
 type fs_env g =
-  restricted_t (x:var{Some? (g x)}) (fun x -> elab_typ (Some?.v (g x)))
+  restricted_t (x:var{Some? (g x)}) (fun x -> get_Type (Some?.v (g x)))
 
 let fs_empty : fs_env empty =
   on_dom
     (x:var{Some? (empty x)})
-    #(fun x -> elab_typ (Some?.v (empty x)))
+    #(fun x -> get_Type (Some?.v (empty x)))
     (fun _ -> assert False)
 
 let get_v #g fs_s x = fs_s x
@@ -16,14 +16,14 @@ let get_v #g fs_s x = fs_s x
 let fs_extend #g fs_s #t fs_v =
   on_dom
     (x:var{Some? ((extend t g) x)})
-    #(fun x -> elab_typ (Some?.v ((extend t g) x)))
+    #(fun x -> get_Type (Some?.v ((extend t g) x)))
     (fun y ->
       if y = 0 then fs_v else fs_s (y-1))
 
 let fs_shrink #t #g fs_s =
   on_dom
     (x:var{Some? (g x)})
-    #(fun x -> elab_typ (Some?.v (g x)))
+    #(fun x -> get_Type (Some?.v (g x)))
     (fun y -> fs_s (y+1))
 
 let lem_fs_extend fs_s v = ()
@@ -33,5 +33,5 @@ let shrink_extend_inverse #g fs_s #t v =
   let fs_s' : fs_env g = fs_shrink (fs_extend fs_s v) in
   assert (forall x. fs_s' x == fs_s x);
   assert (feq fs_s' fs_s);
-  extensionality (x:var{Some? (g x)}) (fun x -> elab_typ (Some?.v (g x))) fs_s' fs_s;
+  extensionality (x:var{Some? (g x)}) (fun x -> get_Type (Some?.v (g x))) fs_s' fs_s;
   assert (fs_s' == fs_s)
