rupicola/stlc_v2/RHC.fst
@@ -5,7 +5,6 @@ open FStar.Tactics.Typeclasses
 
 open STLC
 open SyntacticTypes
-open SemanticTyping
 open EquivRel
 open Compiler
 
@@ -22,10 +21,8 @@ type wholeS = bool // CA: To be able to compile whole programs requires a proof 
 let linkS (#i:intS) (ps:progS i) (cs:ctxS i) : wholeS =
   (dfst ps) cs
 
-type behS_t = bool
-
-val behS : wholeS -> behS_t
-let behS ws = ws
+assume type behS_t
+assume val behS : wholeS -> behS_t
 
 (** Target **)
 
@@ -34,78 +31,62 @@ noeq type intT = { ct : typ }
 val comp_int : intS -> intT
 let comp_int i = { ct = i.comp_ct.t }
 
-type progT (i:intT) = pt:closed_exp{sem_typing empty pt (TArr i.ct TBool)}
-type ctxT (i:intT) = ct:value{sem_typing empty ct i.ct}
-type wholeT = wt:closed_exp{sem_typing empty wt TBool}
+type progT (i:intT) = closed_exp
+type ctxT (i:intT) = ct:value//{sem_typing empty ct i.ct}
+(** CA: syntactic typing necessary so that one can backtranslate and to know the type.
+   **)
+type wholeT = closed_exp
 
 let linkT (#i:intT) (pt:progT i) (ct:ctxT i) : wholeT =
   let wt = EApp pt ct in
-  assume (is_closed wt);
-  assume (sem_typing empty wt TBool);
   wt
 
-assume val eval : t:typ -> e:closed_exp{sem_typing empty e t} -> elab_typ t
-assume val eval_equiv (t:typ) (e:closed_exp{sem_typing empty e t}) : Lemma (t ∋ (eval t e, e))
+assume type behT_t
+assume val behT : wt:wholeT -> behT_t
+assume val rel_behs : behS_t -> behT_t -> Type0
+assume val backtranslate_ctx : (#i:intS) -> ctxT (comp_int i) -> ctxS i
 
-type behT_t = bool
-
-val behT : wt:wholeT -> bool
-let behT wt =
-  eval TBool wt
-
-val rel_behs : behS_t -> behT_t -> Type0
-[@"opaque_to_smt"]
-let rel_behs = (==)
-
+(** CA: I suppose these two lemmas are the most hard core **)
 assume val lem_rel_beh (fs_e: wholeS) (e:wholeT) :
   Lemma
-    (requires TBool ⦂ (fs_e, e))
+    (requires tbool ⦂ (fs_e, e)) (** here it is tbool because whole programs return booleans **)
     (ensures  (behS fs_e) `rel_behs` (behT e))
 
-let compile_prog (#i:intS) (ps:progS i) : progT (comp_int i) =
-  (dsnd ps).typing_proof ();
-  (dsnd ps).e
+assume val lem_bt_ctx i ct : Lemma (pack i.comp_ct ∋ (backtranslate_ctx #i ct, ct))
 
+let compile_prog (#i:intS) (ps:progS i) : progT (comp_int i) =
+  (dsnd ps).e
 
 (** The order of the quantifiers makes this RHC (Robust Hyperproperty Preservation) **)
 let rhc (#i:intS) (ps:progS i) =
   forall (ct:ctxT (comp_int i)).
     exists (cs:ctxS i). behS (linkS ps cs) `rel_behs` behT (linkT (compile_prog ps) ct)
 
-val backtranslate_ctx : (#i:intS) -> ctxT (comp_int i) -> ctxS i
-let backtranslate_ctx #i ct = eval i.comp_ct.t ct
-
 let rhc_1 (#i:intS) (ps:progS i) =
   forall ct. behS (linkS ps (backtranslate_ctx ct)) `rel_behs` behT (linkT (compile_prog ps) ct)
 
 let proof_rhc i ps : Lemma (rhc_1 #i ps) =
   introduce forall ct. behS (linkS ps (backtranslate_ctx ct)) `rel_behs` behT (linkT (compile_prog ps) ct) with begin
-    let t : typ = (comp_int i).ct in
+    let t : typsr = pack (i.comp_ct) in
     let pt : exp = (dsnd ps).e in
-    (dsnd ps).typing_proof ();
     let pt : progT (comp_int i) = pt in
     let ws : wholeS = (dfst ps) (backtranslate_ctx ct) in
     let wt : exp = EApp pt ct in
-    assume (is_closed wt); // is_closed pt /\ is_closed ct ==> is_closed wt
-    assume (sem_typing empty wt TBool);
     let wt : wholeT = wt in
     (dsnd ps).equiv_proof ();
     let ps' = dfst ps in
     lemma_compile_closed_in_equiv_rel ps' #(dsnd ps);
-    assert ((TArr t TBool) ⦂ (ps', pt));
+    assert (mk_arrow t tbool ⦂ (ps', pt));
     lemma_compile_closed_arrow_is_elam #_ #_ #i.comp_ct ps' #(dsnd ps);
     assert (ELam? pt /\ is_closed pt /\ irred pt);
-    eliminate forall (e':closed_exp). steps pt e' ==> irred e' ==> TArr t TBool ∋ (ps', e') with pt;
-    assert (TArr t TBool ∋ (ps', pt)); (** this should be proveable **)
-    eliminate forall (v:value) (fs_v:elab_typ t). t ∋ (fs_v, v) ==>
-        TBool ⦂ (ps' fs_v, subst_beta v (ELam?.b pt))
+    eliminate forall (e':closed_exp). steps pt e' ==> irred e' ==> mk_arrow t tbool ∋ (ps', e') with pt;
+    assert (mk_arrow t tbool ∋ (ps', pt));
+    eliminate forall (v:value) (fs_v:get_Type t). t ∋ (fs_v, v) ==>
+        tbool ⦂ (ps' fs_v, subst_beta v (ELam?.b pt))
       with ct (backtranslate_ctx ct);
-    eval_equiv t ct;
-    assert (TBool ⦂ (ps' (backtranslate_ctx ct), subst_beta ct (ELam?.b pt)));
-    assume (sem_typing empty (subst_beta ct (ELam?.b pt)) TBool);
+    lem_bt_ctx i ct;
+    assert (tbool ⦂ (ps' (backtranslate_ctx ct), subst_beta ct (ELam?.b pt)));
     lem_rel_beh (ps' (backtranslate_ctx ct)) (subst_beta ct (ELam?.b pt));
- //   assert ((ps' (backtranslate_ctx ct) == eval TBool (subst_beta ct (ELam?.b pt))));
     assume (behT (EApp pt ct) == behT (subst_beta ct (ELam?.b pt))); (** simple to prove **)
-//    assert (behS ws == behT wt);
     ()
   end
